michael_formal/not4afp/Drinks_Machine_Payforward.thy
@@ -2,14 +2,14 @@ theory Drinks_Machine_Payforward
   imports "../examples/Drinks_Machine"
 begin
 
-(* This version of drinks_machine supercedes all of those before 03/04/18 *)
-(* It also supercedes "vend.thy"*)
+\<comment>\<open> This version of drinks_machine supercedes all of those before 03/04/18 \<close>
+\<comment>\<open> It also supercedes "vend.thy"\<close>
 
 definition "setup" :: "transition" where
 "setup \<equiv> \<lparr>
         Label = ''setup'',
         Arity = 0,
-        Guard = [], (* No guards *)
+        Guard = [], \<comment>\<open> No guards \<close>
         Outputs = [],
         Updates = [(R 2, (L (Num 0)))]
       \<rparr>"
@@ -18,10 +18,10 @@ definition "select" :: transition where
 "select \<equiv> \<lparr>
         Label = ''select'',
         Arity = 1,
-        Guard = [], (* No guards *)
+        Guard = [], \<comment>\<open> No guards \<close>
         Outputs = [],
         Updates = [
-                    (R 1, (V (I 1))), (*  Firstly set value of r1 to value of i1 *)
+                    (R 1, (V (I 1))), \<comment>\<open>  Firstly set value of r1 to value of i1 \<close>
                     (R 2, (V (R 2)))
                   ]
       \<rparr>"
@@ -30,8 +30,8 @@ definition vend :: "transition" where
 "vend \<equiv> \<lparr>
         Label = ''vend'',
         Arity = 0,
-        Guard = [(Ge (V (R 2)) (L (Num 100)))], (* This is syntactic sugar for ''Not (Lt (V (R 2)) (N 100))'' which could also appear *)
-        Outputs =  [(V (R 1))], (* This has one output o1:=r1 where ''r1'' is a variable with a value *)
+        Guard = [(Ge (V (R 2)) (L (Num 100)))], \<comment>\<open> This is syntactic sugar for ''Not (Lt (V (R 2)) (N 100))'' which could also appear \<close>
+        Outputs =  [(V (R 1))], \<comment>\<open> This has one output o1:=r1 where ''r1'' is a variable with a value \<close>
         Updates = [
                     (R 1, (V (R 1))),
                     (R 2, Minus (V (R 2)) (L (Num 100)))
@@ -40,10 +40,10 @@ definition vend :: "transition" where
 
 definition drinks :: transition_matrix where
 "drinks \<equiv> {|
-             ((0,1), setup),  (* If we want to go from state 0 to state 1 then select will do that *)
-             ((1,2), select), (* If we want to go from state 1 to state 2 then coin will do that *)
-             ((2,2), coin),   (* If we want to go from state 2 to state 2 then drinks will do that *)
-             ((2,1), vend)    (* If we want to go from state 2 to state 1 then drinks will do that *)
+             ((0,1), setup),  \<comment>\<open> If we want to go from state 0 to state 1 then select will do that \<close>
+             ((1,2), select), \<comment>\<open> If we want to go from state 1 to state 2 then coin will do that \<close>
+             ((2,2), coin),   \<comment>\<open> If we want to go from state 2 to state 2 then drinks will do that \<close>
+             ((2,1), vend)    \<comment>\<open> If we want to go from state 2 to state 1 then drinks will do that \<close>
          |}"
 
 lemmas transitions = select_def coin_def vend_def setup_def
@@ -63,8 +63,6 @@ lemma possible_steps_2_coin: "possible_steps drinks 2 d ''coin'' [Num n] = {|(2,
 lemma possible_steps_2_vend: "r (R 2) = Some (Num n) \<Longrightarrow> n \<ge> 100 \<Longrightarrow> possible_steps drinks 2 r ''vend'' [] = {|(1, vend)|}"
   apply (simp add: possible_steps_def drinks_def transitions)
   by force
-
-declare One_nat_def [simp del]
 
 lemma "observe_trace drinks 0 <> [(''setup'', []), (''select'', [Str ''coke'']), (''coin'',[Num 110]), (''vend'', []), (''select'', [Str ''pepsi'']), (''coin'',[Num 90]), (''vend'', [])] = [[],[],[Num 110],[Str ''coke''],[],[Num 100],[Str ''pepsi'']]"
   unfolding observe_trace_def observe_all_def step_def
